working/composition/event_based_refinement/load_balancer/DistributedSystem.t.dfy
@@ -1,0 +1,59 @@
+include "AdditionServiceSpec.t.dfy"
+include "Host.t.dfy"
+include "Network.t.dfy"
+
+abstract module AbstractDistributedSystem {
+    import opened Types
+    import Network
+    import Host: AbstractHost
+
+    datatype Constants = Constants(
+        hosts: seq<Host.Constants>,
+        network: Network.Constants) 
+    {
+        ghost predicate WF() 
+        {
+            Host.GroupWFConstants(hosts)
+        }
+    }
+
+    datatype Variables = Variables(
+        hosts: seq<Host.Variables>,
+        network: Network.Variables) 
+    {
+        ghost predicate WF(c: Constants) {
+            && c.WF()
+            && |c.hosts| == |hosts|
+            && Host.GroupWFVariables(c.hosts, hosts)
+        }
+    }
+
+    ghost predicate Init(c: Constants, v: Variables) {
+        && v.WF(c)
+        && (forall i :: 0 <= i < |c.hosts| ==> Host.Init(c.hosts[i], v.hosts[i]))
+        && Network.Init(c.network, v.network)
+    }
+
+    ghost predicate HostAction(c: Constants, v: Variables, v': Variables, evt: Event, hostId: nat, msgOps: MessageOps)
+    {
+        && v.WF(c)
+        && v'.WF(c)
+        && 0 <= hostId < |v.hosts|
+        && Host.Next(c.hosts[hostId], v.hosts[hostId], v'.hosts[hostId], evt, msgOps)
+        && (forall i :: 0 <= i < |v.hosts| && i != hostId ==> v.hosts[i] == v'.hosts[i])
+        && Network.Next(c.network, v.network, v'.network, msgOps)
+    }
+
+    datatype Step =
+        | HostActionStep(hostId: nat, msgOps: MessageOps)
+
+    ghost predicate NextStep(c: Constants, v: Variables, v': Variables, evt: Event, step: Step)
+    {
+        && HostAction(c, v, v', evt, step.hostId, step.msgOps)
+    }
+
+    ghost predicate Next(c: Constants, v: Variables, v': Variables, evt: Event)
+    {
+        exists step :: NextStep(c, v, v', evt, step)
+    }
+}
