working/composition/event_based_refinement/load_balancer/Host.v.dfy
@@ -1,0 +1,79 @@
+include "AdditionServiceSpec.t.dfy"
+include "Network.t.dfy"
+include "Host.t.dfy"
+include "Client.v.dfy"
+include "Server.v.dfy"
+include "LoadBalancer.v.dfy"
+
+module Host refines AbstractHost {
+    import ClientHost
+    import ServerHost
+    import LoadBalancerHost
+
+    datatype Constants =
+    | ClientConstants(client: ClientHost.Constants)
+    | ServerConstants(server: ServerHost.Constants)
+    | LoadBalancerConstants(loadBalancer: LoadBalancerHost.Constants)
+    {
+        ghost predicate WF() {
+            match this
+            case ClientConstants(c) => c.WF()
+            case ServerConstants(s) => s.WF()
+            case LoadBalancerConstants(l) => l.WF()
+        }
+    }
+
+    datatype Variables =
+    | ClientVariables(client: ClientHost.Variables)
+    | ServerVariables(server: ServerHost.Variables)
+    | LoadBalancerVariables(loadBalancer: LoadBalancerHost.Variables)
+    {
+        ghost predicate WF(c: Constants) {
+            && (ClientVariables? <==> c.ClientConstants?)
+            && (ServerVariables? <==> c.ServerConstants?)
+            && (LoadBalancerVariables? <==> c.LoadBalancerConstants?)
+            && (match c
+                case ClientConstants(_) => client.WF(c.client)
+                case ServerConstants(_) => server.WF(c.server)
+                case LoadBalancerConstants(_) => loadBalancer.WF(c.loadBalancer)
+            )
+        }
+    }
+
+    ghost predicate GroupWFConstants(c: seq<Constants>) {
+        && |c| == 3
+        && c[0].ClientConstants?
+        && c[1].ServerConstants?
+        && c[2].LoadBalancerConstants?
+        && (forall i :: 0 <= i < |c| ==> c[i].WF())
+    }
+
+    ghost predicate GroupWFVariables(c: seq<Constants>, v: seq<Variables>) {
+        && |v| == |c|
+        && GroupWFConstants(c)
+        && (forall i :: 0 <= i < |v| ==> v[i].WF(c[i]))
+    }
+
+    ghost predicate Init(c: Constants, v: Variables) {
+        && v.WF(c)
+        && (match v
+            case ClientVariables(_) => ClientHost.Init(c.client, v.client)
+            case ServerVariables(_) => ServerHost.Init(c.server, v.server)
+            case LoadBalancerVariables(_) => LoadBalancerHost.Init(c.loadBalancer, v.loadBalancer)
+        )
+    }
+
+    ghost predicate Next(c: Constants, v: Variables, v': Variables, evt: Event, msgOps: MessageOps) {
+        && v.WF(c)
+        && v'.WF(c)
+        && (v.ClientVariables? ==> v'.ClientVariables?)
+        && (v.ServerVariables? ==> v'.ServerVariables?)
+        && (v.LoadBalancerVariables? ==> v'.LoadBalancerVariables?)
+        && (match v
+            case ClientVariables(_) => ClientHost.Next(c.client, v.client, v'.client, evt, msgOps)
+            case ServerVariables(_) => ServerHost.Next(c.server, v.server, v'.server, evt, msgOps)
+            case LoadBalancerVariables(_) => LoadBalancerHost.Next(c.loadBalancer, v.loadBalancer, v'.loadBalancer, evt, msgOps)
+        )
+    }
+
+}
