working/composition/event_based_refinement/load_balancer/RefinementProof.v.dfy
@@ -1,0 +1,54 @@
+include "AdditionServiceSpec.t.dfy"
+include "Network.t.dfy"
+include "RefinementObligation.t.dfy"
+include "Client.v.dfy"
+include "Server.v.dfy"
+include "LoadBalancer.v.dfy"
+include "Host.v.dfy"
+include "DistributedSystem.v.dfy"
+
+
+module RefinementProof refines RefinementTheorem {
+    import ClientHost
+    import ServerHost
+    import LoadBalancerHost
+    import Network
+    import DistributedSystem = DistributedSystem
+
+    ghost function ConstantsAbstraction(c: DistributedSystem.Constants) : Spec.Constants
+//        requires c.WF()
+    {
+        Spec.Constants(c.hosts[0].client.x, c.hosts[0].client.y)
+    }
+
+    ghost function VariablesAbstraction(c: DistributedSystem.Constants, v: DistributedSystem.Variables) : Spec.Variables
+//        requires v.WF(c)
+    {
+        Spec.Variables(v.hosts[1].server.sum)
+    }
+
+    ghost predicate Inv(c: DistributedSystem.Constants, v: DistributedSystem.Variables)
+    {
+        && v.WF(c)
+        && (v.hosts[1].server.sum.Some? ==> v.hosts[1].server.sum.value == c.hosts[0].client.x + c.hosts[0].client.y)
+        && (forall msg :: msg in v.network.sentMsgs && msg.ClientRequest? ==> msg == ClientRequest(c.hosts[0].client.x, c.hosts[0].client.y))
+        && (forall msg :: msg in v.network.sentMsgs && msg.LBRequest? ==> msg == LBRequest(c.hosts[0].client.x, c.hosts[0].client.y))
+        && (forall msg :: msg in v.network.sentMsgs && msg.LBResponse? ==> msg == LBResponse(c.hosts[0].client.x + c.hosts[0].client.y))
+        && (forall msg :: msg in v.network.sentMsgs && msg.ClientResponse? ==> msg == ClientResponse(c.hosts[0].client.x + c.hosts[0].client.y))
+    }
+
+    lemma RefinementInit(c: DistributedSystem.Constants, v: DistributedSystem.Variables)
+//        requires DistributedSystem.Init(c, v)
+//        ensures Inv(c, v)
+//        ensures Spec.Init(ConstantsAbstraction(c), VariablesAbstraction(c, v))
+    {
+    }
+
+    lemma RefinementNext(c: DistributedSystem.Constants, v: DistributedSystem.Variables, v': DistributedSystem.Variables, evt: Event)
+//        requires DistributedSystem.Next(c, v, v', evt)
+//        requires Inv(c, v)
+//        ensures Inv(c, v') 
+//        ensures Spec.Next(ConstantsAbstraction(c), VariablesAbstraction(c, v), VariablesAbstraction(c, v'), evt) || (VariablesAbstraction(c, v) == VariablesAbstraction(c, v') && evt == NoOp)
+    {
+    }
+}
